TestVectors/dafny/TestVectors/test/RunMain.dfy
@@ -19,22 +19,40 @@ module {:extern} TestWrappedESDKMain {
   import Time
   import MPL = AwsCryptographyMaterialProvidersTypes
   import MaterialProviders
+  import OsLang
 
   // Test execution directory is different for different runtimes.
   // Runtime should define an extern to return the expected test execution directory.
   method {:extern} GetTestVectorExecutionDirectory() returns (res: string)
 
+  method GetDirPrefix() returns (res: string)
+  {
+    if OsLang.GetLanguageShort() == "Java" {
+      res := "../../";
+    } else {
+      res := GetTestVectorExecutionDirectory();
+    }
+  }
+
+  function method AllowRetry() : Types.NetV4_0_0_RetryPolicy
+  {
+    if OsLang.GetLanguageShort() == "Java" then
+      Types.NetV4_0_0_RetryPolicy.FORBID_RETRY
+    else
+      Types.NetV4_0_0_RetryPolicy.ALLOW_RETRY
+  }
+
   method {:test} RunManifestTests() {
-    // TestGenerateEncryptManifest();
-    // TestEncryptManifest();
-    // TestDecryptManifest();
+    TestGenerateEncryptManifest();
+    TestEncryptManifest();
+    TestDecryptManifest();
   }
 
   // Read encrypt manifests for valid ESDK .NET v4.0.0 messages
   // These messages are expected to successfully decrypt without
   // having to retry.
-  method /*{:test}*/ TestNetRetryFlagVectorsExpectSuccess() {
-    var directory := GetTestVectorExecutionDirectory();
+  method {:test} TestNetRetryFlagVectorsExpectSuccess() {
+    var directory := GetDirPrefix();
     var result := EsdkTestManifests.StartDecryptVectors(
       EsdkManifestOptions.Decrypt(
         manifestPath := directory + "dafny/TestVectors/test/valid-Net-4.0.0/",
@@ -48,43 +66,34 @@ module {:extern} TestWrappedESDKMain {
     expect result.Success?;
   }
 
-  method {:test} TestLargePayload() {
-    var client :- expect WrappedESDK.WrappedESDK();
-
-    var mpl :- expect MaterialProviders.MaterialProviders();
-    var key_input := MPL.CreateRawAesKeyringInput (
-      keyNamespace := "namespace",
-      keyName := "keyname",
-      wrappingKey := [3,3,3,3,3,3,3,3,3,3,3,3,3,3,3,3,3,3,3,3,3,3,3,3,3,3,3,3,3,3,3,3],
-      wrappingAlg := MPL.ALG_AES256_GCM_IV12_TAG16
-    );
-    var keyring :- expect mpl.CreateRawAesKeyring(key_input);
-
-    var plain : seq<uint8> := seq(100000000, _ => 42);
-
-    var time := Time.GetAbsoluteTime();
-    var enc_output :- expect client.Encrypt(
-      Types.EncryptInput (
-        plaintext := plain,
-        keyring := Some(keyring), 
-        algorithmSuiteId := Some(MPL.ALG_AES_256_GCM_HKDF_SHA512_COMMIT_KEY)
+  method {:test} TestPerfManifest() {
+    var directory := GetDirPrefix();
+    var result := EsdkTestManifests.StartEncryptVectors(
+      EsdkManifestOptions.Encrypt(
+        manifestPath := directory + "dafny/TestVectors/test/",
+        manifest := "perf-encrypt-manifest.json",
+        decryptManifestOutput := "dafny/TestVectors/test/perf/",
+        report := EsdkManifestOptions.ReportAll
       )
     );
-    var elapsed := Time.TimeSince(time);
-    Time.PrintTimeLong(elapsed, "Large Encrypt", Some(EsdkTestManifests.LogFileName()));
+    if result.Failure? {
+      print "\nTestPerfManifest Encrypt Failure\n", result.error, "\n";
+    }
+    expect result.Success?;
 
-    time := Time.GetAbsoluteTime();
-    var dec_output :- expect client.Decrypt(
-      Types.DecryptInput (
-        ciphertext := enc_output.ciphertext,
-        keyring := Some(keyring)
+    var result2 := EsdkTestManifests.StartDecryptVectors(
+      EsdkManifestOptions.Decrypt(
+        manifestPath := directory + "dafny/TestVectors/test/perf/",
+        manifestFileName := "decrypt-manifest.json",
+        retryPolicy := AllowRetry(),
+        report := EsdkManifestOptions.ReportAll
       )
     );
-    elapsed := Time.TimeSince(time);
-    Time.PrintTimeLong(elapsed, "Large Decrypt", Some(EsdkTestManifests.LogFileName()));
-
-    expect plain == dec_output.plaintext;
-}
+    if result2.Failure? {
+      print "\nTestPerfManifest Decrypt Failure\n", result2.error, "\n";
+    }
+    expect result2.Success?;
+  }
 
   // Read encrypt manifests for invalid ESDK .NET v4.0.0 messages
   // These messages are expected to fail if retry option is set to FORBID_RETRY
@@ -92,8 +101,8 @@ module {:extern} TestWrappedESDKMain {
   // to correctly pass when this configuration runs the invalid net 4.0.0 tests.
   // The errors that we get back from the MPL are opaque errors, not opaque with text...
   // This means that in dafny code we cannot check the error message :(
-  method /*{:test}*/ TestNetInvalidTestVectorsExpectFailure() {
-    var directory := GetTestVectorExecutionDirectory();
+  method {:test} TestNetInvalidTestVectorsExpectFailure() {
+    var directory := GetDirPrefix();
     var result := EsdkTestManifests.StartDecryptVectors(
       EsdkManifestOptions.Decrypt(
         manifestPath := directory + "dafny/TestVectors/test/invalid-Net-4.0.0/",
@@ -107,13 +116,17 @@ module {:extern} TestWrappedESDKMain {
     expect result.Failure?;
   }
 
-  method /*{:test}*/ TestNetInvalidTestVectorsExpectSuccessOnRetry() {
-    var directory := GetTestVectorExecutionDirectory();
+  method {:test} TestNetInvalidTestVectorsExpectSuccessOnRetry() {
+    // we can't retry in Java
+    if OsLang.GetLanguageShort() == "Java" {
+      return;
+    }
+    var directory := GetDirPrefix();
     var result := EsdkTestManifests.StartDecryptVectors(
       EsdkManifestOptions.Decrypt(
         manifestPath := directory + "dafny/TestVectors/test/invalid-Net-4.0.0/",
         manifestFileName := "manifest.json",
-        retryPolicy := Types.NetV4_0_0_RetryPolicy.ALLOW_RETRY
+        retryPolicy := AllowRetry()
       )
     );
     if result.Failure? {
@@ -122,8 +135,8 @@ module {:extern} TestWrappedESDKMain {
     expect result.Success?;
   }
 
-  method /*{:test}*/ TestNet401ValidTestVectorsExpectSuccess() {
-    var directory := GetTestVectorExecutionDirectory();
+  method {:test} TestNet401ValidTestVectorsExpectSuccess() {
+    var directory := GetDirPrefix();
     var result := EsdkTestManifests.StartDecryptVectors(
       EsdkManifestOptions.Decrypt(
         manifestPath := directory + "dafny/TestVectors/test/v4-Net-4.0.1/",
@@ -138,7 +151,7 @@ module {:extern} TestWrappedESDKMain {
   }
 
   method TestGenerateEncryptManifest() {
-    var directory := GetTestVectorExecutionDirectory();
+    var directory := GetDirPrefix();
     var result := WriteVectors.WriteTestVectors(
       EsdkManifestOptions.EncryptManifest(
         encryptManifestOutput := directory + "dafny/TestVectors/test/",
@@ -151,12 +164,13 @@ module {:extern} TestWrappedESDKMain {
   }
 
   method TestEncryptManifest() {
-    var directory := GetTestVectorExecutionDirectory();
+    var directory := GetDirPrefix();
     var result := EsdkTestManifests.StartEncryptVectors(
       EsdkManifestOptions.Encrypt(
         manifestPath := directory + "dafny/TestVectors/test/",
         manifest := "encrypt-manifest.json",
-        decryptManifestOutput := directory + "dafny/TestVectors/test/"
+        decryptManifestOutput := directory + "dafny/TestVectors/test/",
+        report := EsdkManifestOptions.ReportFinal
       )
     );
     if result.Failure? {
@@ -167,12 +181,13 @@ module {:extern} TestWrappedESDKMain {
 
   method TestDecryptManifest()
   {
-    var directory := GetTestVectorExecutionDirectory();
+    var directory := GetDirPrefix();
     var result := EsdkTestManifests.StartDecryptVectors(
       EsdkManifestOptions.Decrypt(
         manifestPath := directory + "dafny/TestVectors/test/",
         manifestFileName := "decrypt-manifest.json",
-        retryPolicy := Types.NetV4_0_0_RetryPolicy.FORBID_RETRY
+        retryPolicy := Types.NetV4_0_0_RetryPolicy.FORBID_RETRY,
+        report := EsdkManifestOptions.ReportFinal
       )
     );
 
